\begin{enumerate}[label=\thesubsection.\arabic*.,ref=\thesubsection.\theenumi]
\numberwithin{equation}{enumi}

\item
Consider the system described by the following state space representation  
\begin{align}
\dot{\vec{ x}}&=\myvec{0&1\\0&-2}\vec{x} + \myvec{0\\1}\vec{u}\\  
\vec{y} &= \myvec{1&0}\vec{x}
\end{align}
If u(t) is a unit step input and 
\begin{align}
\vec{x}(0)=\myvec{x_{1}(0)\\x_{2}(0)}=\myvec{1\\0}
\end{align}
Find the output $y(1)$.
\\
\solution From \ref{eq:ee18btech11006_yx_init}
%
%
\begin{multline}
\vec{Y}(s)=( \vec{C}{(s\vec{I}-\vec{A})^{-1}}\vec{B}+\vec{D}) \vec{U}(s) 
\\
+ \vec{C}(s\vec{I}-\vec{A})^{-1}\vec{x}(0)
\label{eq:ee18btech11006_yx_init}
\end{multline}
%
where
\begin{align}
\vec{A}&=\myvec{0&1\\0&-2}\\
\vec{B}&=\myvec{0\\1}\\
\vec{C}&=\myvec{1&0}\\
\vec{D}&=\myvec{0&0}\\
\vec{x}(0)&=\myvec{1\\0}
\end{align}
%

The following code computes 
\begin{lstlisting}
codes/ee18btech11047.py
\end{lstlisting}
\begin{align}
{Y}(s)&=\frac{s^{2}+2s+1}{s^{3}+2s^{2}}
\\
\implies y(t)&=\brak{\frac{1}{4}e^{-2t}+\frac{3}{4}+\frac{1}{2}t}u(t)
\\
\text{or, } y(1) &= \frac{1}{4}\brak{5 + e^{-2}}
\end{align}
\end{enumerate}
